\documentclass[]{article}
\usepackage{amsmath}
\usepackage{amsfonts}
\usepackage{amssymb}
\usepackage{natbib}
\usepackage[a4paper, margin=1in]{geometry}

%opening
\title{Legendre Polynomials}
\author{Matt James}

\begin{document}

\maketitle


\section{Legendre Polynomials}

	This is the form of a Legendre polynomial (Rodrigues' formula):
	
	\begin{equation}
		P_n(x) = \frac{1}{2^n n!}\frac{\text{d}^n}{\text{d}x^n}(v^2 - 1)^n
	\end{equation}

	where $n$ is the degree of the polynomial. The first 5 degrees (0-4) are shown below:
	
	\begin{align}
		P_0(x) &= \frac{\text{d}^0}{\text{d}x^0} (x^2 - 1)^0 &= 1, \label{EqP0} \\
		P_1(x) &= \frac{1}{2} \frac{\text{d}}{\text{d}x} (x^2 - 1) &= x, \label{EqP1} \\
		P_2(x) &= \frac{1}{8} \frac{\text{d}^2}{\text{d}x^2} (x^2 - 1)^2 &= \frac{1}{2}(3x^2 - 1), \label{EqP2} \\
		P_3(x) &= \frac{1}{48} \frac{\text{d}^3}{\text{d}x^3} (x^2 - 1)^3 &= \frac{1}{2}(5x^3 - 3x), \label{EqP3} \\
		P_4(x) &= \frac{1}{384} \frac{\text{d}^4}{\text{d}x^4} (x^2 - 1)^4 &= \frac{1}{8}(35x^4 - 30x^2 + 3), \label{EqP4}
	\end{align}
	where $x$ can be substituted for $\cos{\theta}$:
	
	\begin{align}
		P_0(\cos{\theta}) &= 1 \label{EqP0t}, \\
		P_1(\cos{\theta}) &= \cos{\theta}, \label{EqP1t} \\
		P_2(\cos{\theta}) &= \frac{1}{2}(3\cos^2{\theta} - 1 \label{EqP2t}), \\
		P_3(\cos{\theta}) &= \frac{1}{2}(5\cos^3{\theta} - 3\cos{\theta}), \label{EqP3t} \\
		P_4(\cos{\theta}) &= \frac{1}{8}(35\cos^4{\theta} - 30x^2 + 3). \label{EqP4t}		
	\end{align}
	
	\subsection{Derivatives}
		
		These derivatives of the above equations \ref{EqP0}--\ref{EqP4} with respect to $x$ will come in handy later on...
		
		For equation \ref{EqP0}:
		
		\begin{align}
			\frac{\text{d}}{\text{d} x}P_0 (x) &= 0. \label{Eqd1P0}
		\end{align}

		For equation \ref{EqP1}:

		\begin{align}
			\frac{\text{d}}{\text{d} x} P_1 (x) &= 1. \label{Eqd1P1}
		\end{align}
		
		For equation \ref{EqP2}:

		\begin{align}
			\frac{\text{d}}{\text{d} x} P_2 (x) &= 3x, \label{Eqd1P2} \\
			\frac{\text{d}^2}{\text{d} x^2} P_2 (x) &= 3. \label{Eqd2P2}
		\end{align}
		
		For equation \ref{EqP3}:
		
		\begin{align}
			\frac{\text{d}}{\text{d} x} P_3 (x) &= \frac{1}{2}(15x^2 - 3), \label{Eqd1P3} \\
			\frac{\text{d}^2}{\text{d} x^2} P_3 (x) &= 15x, \label{Eqd2P3} \\
			\frac{\text{d}^3}{\text{d} x^3} P_3 (x) &= 15. \label{Eqd3P3}
		\end{align}
		
		For equation \ref{EqP4}:

		\begin{align}
			\frac{\text{d}}{\text{d} x} P_4 (x) &= \frac{5}{2}(7x^3 - 3x), \label{Eqd1P4} \\
			\frac{\text{d}^2}{\text{d} x^2} P_4 (x) &= \frac{15}{2}(7x^2 - 1), \label{Eqd2P4} \\
			\frac{\text{d}^3}{\text{d} x^3} P_4 (x) &= 105x, \label{Eqd3P4} \\
			\frac{\text{d}^4}{\text{d} x^4} P_4 (x) &= 105. \label{Eqd4P4}
		\end{align}
			
\section{Ferrers Normalized Legendre Polynomials}

	The Ferrers normalized Legendre polynomials are defined by \cite{Ferrers1877} as:
	
	\begin{equation}
		P_{n,m}(x) = (1 - x^2)^\frac{m}{2} \frac{\text{d}^m}{\text{d}x^m} P_n(x) \label{EqFerrers},
	\end{equation}
	where $m$ is the order.


	Some equations and their derivatives...
	
	\begin{align}
		P_{0,0} (x) &= 1, \\
		P_{0,0} (\cos{\theta}) &= 1, \\
		\frac{\text{d}}{\text{d} \theta} P_{0,0} &= 0.
	\end{align}

	\begin{align}
		P_{1,0} (x) &= x, \\
		P_{1,0} (\cos{\theta}) &= \cos{\theta}, \\
		\frac{\text{d}}{\text{d} \theta} P_{1,0} &= -\sin{\theta}.
	\end{align}
	
	\begin{align}
		P_{1,1} (x) &= (1 - x^2)^\frac{1}{2}, \\
		P_{1,1} (\cos{\theta}) &= \sin{\theta}, \\
		\frac{\text{d}}{\text{d} \theta} P_{1,1} &= \cos{\theta}.
	\end{align}

	
	\begin{align}
		P_{2,0} (x) &= \frac{1}{2} (3 x^2 - 1), \\
		P_{2,0} (\cos{\theta}) &= \frac{1}{2}(3\cos^2{\theta} - 1), \\
		\frac{\text{d}}{\text{d} \theta} P_{2,0} &= -3\cos{\theta}\sin{\theta}.
	\end{align}

	\begin{align}
		P_{2,1} (x) &= 3x(1-x^2)^\frac{1}{2}, \\
		P_{2,1} (\cos{\theta}) &= 3\cos{\theta}\sin{\theta}, \\
		\frac{\text{d}}{\text{d} \theta} P_{2,1} &= 3(2\cos^2{\theta}-1).
	\end{align}

	\begin{align}
		P_{2,2} (x) &= 3(1-x^2), \\
		P_{2,2} (\cos{\theta}) &= 3\sin^2{\theta}, \\
		\frac{\text{d}}{\text{d} \theta} P_{2,2} &= 6\sin{\theta}\cos{\theta}.
	\end{align}

	\begin{align}
		P_{3,0} (x) &= \frac{1}{2} (5x^3 - 3x), \\
		P_{3,0} (\cos{\theta}) &= \frac{1}{2} (5 \cos^3{\theta} - 3\cos{\theta}), \\
		\frac{\text{d}}{\text{d} \theta} P_{3,0} &= \frac{3}{2} \sin{\theta} (1 - 5 \cos^2{\theta}).
	\end{align}


	\begin{align}
		P_{3,1} (x) &= \frac{1}{2} \sqrt{(1-x^2)}(15x^2 - 3), \\
		P_{3,1} (\cos{\theta}) &= \frac{3}{2} \sin{\theta}(5\cos^2{\theta} -1), \\
		\frac{\text{d}}{\text{d} \theta} P_{3,1} &= \frac{3}{2} \left[\sin{\theta}\frac{\text{d}}{\text{d}\theta}(5\cos^2{\theta}-1) + (5\cos^2{\theta} - 1)\frac{\text{d}}{\text{d}\theta}\sin{\theta}\right], \\
		&= \frac{3}{2} (15\cos^3{\theta} - 11\cos{\theta}).
	\end{align}

	\begin{align}
		P_{3,2} (x) &= 15x (1-x^2), \\
		P_{3,2} (\cos{\theta}) &= 15 \cos{\theta} \sin^2{\theta}, \\
		\frac{\text{d}}{\text{d} \theta} P_{3,2} &= 15 \sin{\theta} (3\cos^2{\theta} - 1).
	\end{align}

	\begin{align}
		P_{3,3} (x) &= 15(1-x^2)^\frac{3}{2}, \\
		P_{3,3} (\cos{\theta}) &= 15 \sin^3{\theta}, \\
		\frac{\text{d}}{\text{d} \theta} P_{3,3} &= 45 \sin^2{\theta}\cos{\theta}.
	\end{align}

	\begin{align}
		P_{4,0} (x) &= \frac{1}{8}(35x^4 - 30x^2 + 3), \\
		P_{4,0} (\cos{\theta}) &= \frac{1}{8}(35 \cos^4{\theta} - 30\cos^2{\theta} + 3), \\
		\frac{\text{d}}{\text{d} \theta} P_{4,0} &= \frac{5}{2}(7\cos^3{\theta} - 3\cos{\theta}).
	\end{align}


	\begin{align}
		P_{4,1} (x) &= \frac{5}{2}(7x^3 - 3x) (1-x^2)^\frac{1}{2}, \\
		P_{4,1} (\cos{\theta}) &= \frac{5}{2} \sin{\theta}(7\cos^3{\theta} - 3\cos{\theta}), \\
		\frac{\text{d}}{\text{d} \theta} P_{4,1} &= \frac{5}{2}\left[(7\cos^3{\theta} - 3\cos{\theta})\frac{\text{d}}{\text{d}\theta}\sin{\theta} + \sin{\theta} \frac{\text{d}}{\text{d}\theta}(7\cos^3{\theta} - 3\cos{\theta})\right], \\
		&= \frac{5}{2}(28 \cos^4{\theta} - 27 \cos^3{\theta} + 3).
	\end{align}
	


	\begin{align}
		P_{4,2} (x) &= \frac{15}{2}(7x^2 - 1) (1-x^2), \\
		P_{4,2} (\cos{\theta}) &= \frac{15}{2} \sin^2{\theta}(7\cos^2{\theta} - 1), \\
		\frac{\text{d}}{\text{d} \theta} P_{4,2} &= \frac{15}{2}\left[(7\cos^2{\theta} - 1)\frac{\text{d}}{\text{d}\theta}\sin^2{\theta} + \sin^2{\theta} \frac{\text{d}}{\text{d}\theta}(7\cos^2{\theta} - 1)\right], \\
		&= 30\cos{\theta}\sin{\theta}(7\cos^2{\theta} - 4).
	\end{align}

	\begin{align}
		P_{4,3} (x) &= 105x(1-x^2)^\frac{3}{2}, \\
		P_{4,3} (\cos{\theta}) &= 105 \cos{\theta}\sin^3{\theta}, \\
		\frac{\text{d}}{\text{d} \theta} P_{4,3} &= 105\left[\cos{\theta}\frac{\text{d}}{\text{d}\theta}\sin^3{\theta} + \sin^3{\theta}\frac{\text{d}}{\text{d}\theta}\cos{\theta}\right], \\
		&= 105 \sin^2{\theta}(4\cos^2{\theta} - 1).
	\end{align}	

	\begin{align}
		P_{4,4} (x) &= 105(1-x^2)^2, \\
		P_{4,4} (\cos{\theta}) &= 105 \sin^4{\theta}, \\
		\frac{\text{d}}{\text{d} \theta} P_{4,4} &= 420 \sin^3{\theta} \cos{\theta}.
	\end{align}	
	
	\subsection{Recurrence Relations}
	
		There are three recurrence relations which can be used to calculate the associate polynomials from lower order/degree polynomials.
		
		\begin{align}
			&\text{A: }  m < n-1  \nonumber \\ 
			&P_{n,m} (\cos{\theta}) = \frac{1}{n-m} \left[(2n-1)\cos{\theta} P_{n-1,m} - (n + m -1)P_{n-2,m}\right] \\
			&\text{B: }  m = n-1  \nonumber \\ 
			&P_{n,m} (\cos{\theta}) = (2n-1)\sin{\theta} P_{n-1,m-1}, \\
			&\text{C: }  m = n  \nonumber \\ 
			&P_{n,m} (\cos{\theta}) = (2n-1)\sin{\theta} P_{n-1,m-1}.
		\end{align}
		
		Examples for case A:
		
		\begin{align}
			P_{2,0} &= \frac{1}{2}\left[ 3\cos{\theta} P_{1,0} - P_{0,0} \right] \\
					&= \frac{1}{2}(3\cos^2{\theta} - 1) \\
			P_{3,0} &= \frac{1}{3}\left[5\cos{\theta}P_{2,0} - 2P_{1,0}\right] \\
					&= \frac{1}{2}(5 \cos^3{\theta} - 3\cos{\theta}) \\
			P_{3,1} &= \frac{1}{2}\left[5 \cos{\theta} P_{2,1} - 3P_{1,1}\right] \\
					&= \frac{3}{2}\sin{\theta}\left[5 \cos^2{\theta} - 1\right] \\
			P_{4,0} &= \frac{1}{4}\left[7\cos{\theta}P_{3,0} - 3P_{2,0}\right] \\
					&= \frac{1}{8}(35 \cos^4{\theta} - 30\cos^2{\theta} + 3) \\
			P_{4,1} &= \frac{1}{3}\left[7\cos{\theta} P_{3,1} - 4P_{2,1}\right] \\
					&= \frac{5}{2}\sin{\theta}\cos{\theta}(7\cos^2{\theta} - 3) \\
			P_{4,2} &= \frac{1}{2}\left[7\cos{\theta}P_{3,2} - 5P_{2,2}\right] \\
					&= \frac{15}{2}\sin^2{\theta}(7\cos^2{\theta} -1)
		\end{align}
		
		Examples for case B:
		
		\begin{align}
			P_{2,1} &= 3\sin{\theta}P_{1,0} \\
					&= 3\sin{\theta}\cos{\theta} \\
			P_{3,2} &= 5\sin{\theta}P_{2,1} \\
					&= 15\sin^2{\theta}\cos{\theta} \\
			P_{4,3} &= 7\sin{\theta}P_{3,2} \\
					&= 105\sin^3{\theta}\cos{\theta} 
		\end{align}
		
		Examples for case C (I think this rule is basically the same as B):
		
		\begin{align}
			P_{1,1} &= \sin{\theta}P_{0,0} \\
					&= \sin{\theta} \\
			P_{2,2} &= 3\sin{\theta}P_{1,1} \\
					&= 3\sin^2{\theta} \\
			P_{3,3} &= 5\sin{\theta}P_{2,2} \\
					&= 15\sin^3{\theta} \\
			P_{4,4} &= 7\sin{\theta}P_{3,3} \\
					&= 105\sin^4{\theta}
		\end{align}
		
		The derivatives can be calculated using similar rules:
		
		\begin{align}
			&\text{A: }  m < n-1  \nonumber \\ 
			&\frac{\text{d}}{\text{d}\theta} P_{n,m} = \frac{1}{n-m} \left[(2n-1)\left(\cos{\theta}\frac{\text{d}}{\text{d}\theta}P_{n-1,m} - \sin{\theta}P_{n-1,m}\right) - (n+m-1)\frac{\text{d}}{\text{d}\theta}P_{n-2,m}\right] \\
			&\text{B: }  m = n-1  \nonumber \\ 
			&\frac{\text{d}}{\text{d}\theta} P_{n,m} = (2n-1) \left[\sin{\theta}\frac{\text{d}}{\text{d}\theta}P_{n-1,m-1} + \cos{\theta}P_{n-1,m-1}\right] \\
			&\text{C: }  m = n  \nonumber \\ 
			&\frac{\text{d}}{\text{d}\theta} P_{n,m} = (2n-1) \left[\sin{\theta}\frac{\text{d}}{\text{d}\theta}P_{n-1,m-1} + \cos{\theta}P_{n-1,m-1}\right]
		\end{align}
		
		Examples for case A:
		
		\begin{align}
			\frac{\text{d}}{\text{d}\theta}P_{2,0} &= \frac{1}{2}\left[3\left(\cos{\theta}\frac{\text{d}}{\text{d}\theta}P_{1,0} - \sin{\theta}P_{1,0}\right) - \frac{\text{d}}{\text{d} \theta} P_{0,0}\right] \\
				&= \frac{1}{2} (3 \cos^2{\theta} -1)\\
			\frac{\text{d}}{\text{d}\theta}P_{3,0} &= \frac{1}{3}\left[5\left(\cos{\theta}\frac{\text{d}}{\text{d}\theta}P_{2,0} - \sin{\theta}P_{2,0}\right) - 2\frac{\text{d}}{\text{d} \theta} P_{1,0}\right] \\
				&= \frac{1}{2}(5\cos^3{\theta} - 3\cos{\theta})\\
			\frac{\text{d}}{\text{d}\theta}P_{3,1} &= \frac{1}{2}\left[5\left(\cos{\theta}\frac{\text{d}}{\text{d}\theta}P_{2,1} - \sin{\theta}P_{2,1}\right) - 3\frac{\text{d}}{\text{d} \theta} P_{1,1}\right] \\
				&= \frac{3}{2}\sin{\theta}(5\cos^2{\theta} - 1)\\
			\frac{\text{d}}{\text{d}\theta}P_{4,0} &= \frac{1}{4}\left[7\left(\cos{\theta}\frac{\text{d}}{\text{d}\theta}P_{3,0} - \sin{\theta}P_{3,0}\right) - 3\frac{\text{d}}{\text{d} \theta} P_{2,0}\right] \\
				&= \frac{1}{8}(35\cos^4{\theta} - 30\cos^2{\theta} + 3)\\
			\frac{\text{d}}{\text{d}\theta}P_{4,1} &= \frac{1}{3}\left[7\left(\cos{\theta}\frac{\text{d}}{\text{d}\theta}P_{3,1} - \sin{\theta}P_{3,1}\right) - 4\frac{\text{d}}{\text{d} \theta} P_{2,1}\right] \\
				&= \frac{5}{2} \sin{\theta}\cos{\theta}(7\cos^2{\theta} - 3) \\
			\frac{\text{d}}{\text{d}\theta}P_{4,2} &= \frac{1}{2}\left[7\left(\cos{\theta}\frac{\text{d}}{\text{d}\theta}P_{3,2} - \sin{\theta}P_{3,2}\right) - 5\frac{\text{d}}{\text{d} \theta} P_{2,2}\right] \\
				&= \frac{15}{2}\sin^2{\theta}(7\cos^2{\theta} - 1)
		\end{align}
		
		Examples for case B:
		
		\begin{align}
			\frac{\text{d}}{\text{d}\theta}P_{2,1} &= 3 \left[\sin{\theta}\frac{\text{d}}{\text{d}\theta}P_{1,0} + \cos{\theta}P_{1,0}\right] \\
			&= 6 \cos^2{\theta} - 3\\
			\frac{\text{d}}{\text{d}\theta}P_{3,2} &= 5 \left[\sin{\theta}\frac{\text{d}}{\text{d}\theta}P_{2,1} + \cos{\theta}P_{2,1}\right] \\
			&= 15\sin{\theta}(3\cos^2{\theta} -1)\\
			\frac{\text{d}}{\text{d}\theta}P_{4,3} &= 7 \left[\sin{\theta}\frac{\text{d}}{\text{d}\theta}P_{3,2} + \cos{\theta}P_{3,2}\right] \\
			&= 105\sin^2{\theta}(4\cos^2{\theta} - 1)
		\end{align}

		Examples for case C:
		
		\begin{align}
			\frac{\text{d}}{\text{d}\theta}P_{2,2} &= 3 \left[\sin{\theta}\frac{\text{d}}{\text{d}\theta}P_{1,1} + \cos{\theta}P_{1,1}\right] \\
			&= 6 \cos{\theta}\sin{\theta} \\
			\frac{\text{d}}{\text{d}\theta}P_{3,3} &= 5 \left[\sin{\theta}\frac{\text{d}}{\text{d}\theta}P_{2,2} + \cos{\theta}P_{2,2}\right] \\
			&= 45\cos{\theta}\sin^2{\theta}\\
			\frac{\text{d}}{\text{d}\theta}P_{4,4} &= 7 \left[\sin{\theta}\frac{\text{d}}{\text{d}\theta}P_{3,3} + \cos{\theta}P_{3,3}\right] \\
			&= 420\cos{\theta}\sin^3{\theta}
		\end{align}
		
	
		The recurrence relations listed above can be used to calculate any of the associated Legendre polynomials provided that $P_{0,0}$, $P_{1,0}$ and $P_{1,1}$ are defined initially. Here are some examples below, where the left polynomial is formed using the polynomial(s) to the right of the arrow and the letter in brackets corresponds to the three rules listed above:
		
		\begin{align}
			P_{2,0} &\leftarrow P_{1,0},P_{0,0} &(C) \\
			P_{2,1} &\leftarrow P_{1,0}			&(B) \\
			P_{2,2} &\leftarrow P_{1,1}			&(A) \\
			\nonumber \\
			P_{3,0} &\leftarrow P_{2,0},P_{1,0} &(C) \\
			P_{3,1} &\leftarrow P_{2,1},P_{1,1} &(C) \\
			P_{3,2} &\leftarrow P_{2,1}			&(B) \\
			P_{3,3} &\leftarrow P_{2,2}			&(A) \\
			\nonumber \\
			P_{4,0} &\leftarrow P_{3,0},P_{2,0} &(C) \\
			P_{4,1} &\leftarrow P_{3,1},P_{2,1} &(C) \\
			P_{4,2} &\leftarrow P_{3,2},P_{2,2} &(C) \\
			P_{4,3} &\leftarrow P_{3,2}			&(B) \\
			P_{4,4} &\leftarrow P_{3,3}			&(A) 
		\end{align}
	
		Note that the same rules apply for the derivatives too.
		
\section{Schmidt Normalized Legendre Polynomials}
	
	The Schmidt normalized Legendre polynomials, $P_n^m$, are defined by
	
	\begin{equation}
		P_n^m = S_n^m P_{n,m},
	\end{equation}
	
	where 
	
	\begin{equation}
		S_{n,m} = \sqrt{(2-\delta_m^0)\frac{(n-m)!}{(n+m)!}},
	\end{equation}
	
	and $\delta_m^0 = 1$ when $m = 0$, and is $\delta_m^0 = 0$ otherwise.
\bibliographystyle{agufull08}
\bibliography{ref}
\end{document}
